examples/map/MapI.v
@@ -7,6 +7,7 @@ Require Import Skeleton.
 Require Import MapHeader.
 Require Import PCM.
 Require Import STB IPM ITactics.
+Require Import MemHeader.
 
 
 Require Import sProp sWorld World SRF.
@@ -35,18 +36,21 @@ Module MapI.
 Section I.
   Local Open Scope string_scope.
   Context `{_W: CtxWD.t}.
+
+  Definition scope := "Map".
+  Definition v_hptr := scope ↯ "hptr".
   
   Definition init: list val -> itree pmodE val :=
     fun varg =>
       `sz: Z <- (pargs [Tint] varg)?;;
-      `hptr: val <- ccallU "alloc" [Vint sz];;
-      trigger (SPut "hptr" hptr↑);;;
+      `hptr: val <- ccallU MemName.alloc [Vint sz];;
+      cput v_hptr hptr↑;;;
       (ITree.iter
          (fun i =>
             if (Z_lt_le_dec i sz)
             then
               vptr <- (vadd hptr (Vint (i * 8)))?;;
-              `_: val <- ccallU "store" [vptr; Vint 0];;
+              `_: val <- ccallU MemName.store [vptr; Vint 0];;
               Ret (inl (i + 1)%Z)
             else
               Ret (inr tt)) 0%Z);;;
@@ -56,18 +60,18 @@ Section I.
   Definition get: list val -> itree pmodE val :=
     fun varg =>
       k <- (pargs [Tint] varg)?;;
-      hptr <- trigger (SGet "hptr");; hptr <- hptr↓?;;
+      hptr <- cgetU v_hptr;;
       vptr <- (vadd hptr (Vint (k * 8)))?;;
-      `r: val <- ccallU "load" [vptr];; r <- (unint r)?;;
+      `r: val <- ccallU MemName.load [vptr];; r <- (unint r)?;;
       Ret (Vint r)
   .
 
   Definition set: list val -> itree pmodE val :=
     fun varg =>
       '(k, v) <- (pargs [Tint; Tint] varg)?;;
-      hptr <- trigger (SGet "hptr");; hptr <- hptr↓?;;
+      hptr <- cgetU v_hptr;; 
       vptr <- (vadd hptr (Vint (k * 8)))?;;
-      `_: val <- ccallU "store" [vptr; Vint v];;
+      `_: val <- ccallU MemName.store [vptr; Vint v];;
       Ret Vundef
   .
 
@@ -79,17 +83,18 @@ Section I.
   .
 
   Definition fnsems :=
-    [(MapName.init, (["hptr"], cfunU init));
-     (MapName.get,  (["hptr"], cfunU get));
-     (MapName.set,  (["hptr"], cfunU set));
-     (MapName.set_by_user, (["hptr"], cfunU set_by_user))].
+    [(MapName.init, ([scope], cfunU init));
+     (MapName.get,  ([scope], cfunU get));
+     (MapName.set,  ([scope], cfunU set));
+     (MapName.set_by_user, ([scope], cfunU set_by_user))].
   
   Program Definition Sem: PModSem.t := {|
+    PModSem.scopes := [scope];
     PModSem.fnsems := fnsems;
-    PModSem.initial_st := [("hptr",tt↑)];
+    PModSem.initial_st := [(v_hptr,tt↑)];
   |}
   .
-  Next Obligation. prove_scope. Qed.
+  Solve All Obligations with prove_scope.
 
   Definition Mod: PMod.t := {|
     PMod.get_modsem := fun _ => Sem;
