examples/map/MapHeader.v
@@ -4,8 +4,8 @@ Require Import Events Any IPM ImpPrelude.
 Module MapName.
   
 Definition init := "Map.init".
-Definition get := "Map.get".
-Definition set := "Map.set".
+Definition get  := "Map.get".
+Definition set  := "Map.set".
 Definition set_by_user := "Map.set_by_user".
 
 End MapName.
