examples/map/MapMAproof.v
@@ -17,7 +17,7 @@ From ExtLib Require Import
      Data.Map.FMapAList.
 
 Require Import STB.
-Require Import Mem1.
+Require Import.
 
 
 Require Import ISim.
