examples/map/MapMSpec.v
@@ -10,7 +10,7 @@ From ExtLib Require Import
      Structures.Maps
      Data.Map.FMapAList.
 Require Import ISim.
-Require Import MapHeader Mem1.
+Require Import MapHeader.
 Require Import sProp sWorld World SRF.
 From stdpp Require Import coPset gmap namespaces.
 Set Implicit Arguments.
@@ -59,12 +59,6 @@ Section MAP.
                     (fun varg => (⌜varg = ([Vint k])↑⌝)%I),
                     (fun vret => True%I)))).  
 
-  Definition fnsems: list (string * fspecbody) :=
-    [(MapName.init, init_spec);
-     (MapName.get, get_spec);
-     (MapName.set, set_spec);
-     (MapName.set_by_user, set_by_user_spec)]
-  
   Definition Stb: alist gname fspec :=
     Seal.sealing "stb" [(MapName.init, init_spec);
                         (MapName.get, get_spec);
