imp_system/mem/MemHeader.v
@@ -1,0 +1,12 @@
+Require Import Coqlib ITreelib sflib.
+Require Import Events Any IPM ImpPrelude.
+
+Module MemName.
+  
+Definition alloc := "Mem.alloc".
+Definition free  := "Mem.free".
+Definition load  := "Mem.load".
+Definition store := "Mem.store".
+Definition cmp   := "Mem.cmp".
+
+End MemName.
