imp_system/mem/MemI.v
@@ -1,0 +1,103 @@
+Require Import Coqlib.
+Require Import ITreelib.
+Require Import ImpPrelude.
+Require Import STS.
+Require Import Behavior.
+Require Import PMod HMod Events.
+Require Import Skeleton.
+Require Import PCM IPM ITactics.
+Require Import MemHeader.
+
+Set Implicit Arguments.
+Set Typeclasses Depth 5.
+
+Module MemI.
+Section MEMI.  
+  (* Let memRA: URA.t := (RA.excl Mem.t). *)
+  (* Context `{@GRA.inG memRA Σ}. *)
+  (* Let GURA: URA.t := GRA.to_URA Σ. *)
+  (* Local Existing Instance GURA. *)
+  (* Compute (URA.car (t:=memRA)). *)
+
+  Definition scope := "Mem".
+  Definition v_mem := scope ↯ "mem".
+
+  Definition alloc: (list val) -> itree pmodE val :=
+    fun varg =>
+      `sz: Z <- (pargs [Tint] varg)?;;
+      mem <- trigger (SGet v_mem);; mem <- mem↓?;;
+      if (Z_le_gt_dec 0 sz && Z_lt_ge_dec (8 * sz) modulus_64)
+      then (delta <- trigger (Choose _);;
+            let mem0: Mem.t := Mem.mem_pad mem delta in
+            let (blk, mem1) := Mem.alloc mem0 sz in
+            trigger (SPut v_mem mem1↑);;;
+            Ret (Vptr blk 0))
+      else triggerUB
+  .
+
+  Definition free: list val -> itree pmodE val :=
+    fun varg =>
+      '(b, ofs) <- (pargs [Tptr] varg)?;;        
+      mem <- trigger (SGet v_mem);; mem <- mem↓?;;
+      mem1 <- (Mem.free mem b ofs)?;;
+      trigger (SPut v_mem mem1↑);;;
+      Ret (Vint 0)
+  .
+
+  Definition load: list val -> itree pmodE val :=
+    fun varg =>
+      '(b, ofs) <- (pargs [Tptr] varg)?;;        
+      mem <- trigger (SGet v_mem);; mem <- mem↓?;;
+      v <- (Mem.load mem b ofs)?;;
+      Ret v
+  .
+
+  Definition store: list val -> itree pmodE val :=
+    fun varg =>
+      '(b, ofs, v) <- (pargs [Tptr; Tuntyped] varg)?;;
+      mem <- trigger (SGet v_mem);; mem <- mem↓?;;
+      mem1 <- (Mem.store mem b ofs v)?;;
+      trigger (SPut v_mem mem1↑);;;
+      Ret (Vint 0)
+  .
+
+  Definition cmp: list val -> itree pmodE val :=
+    fun varg =>
+      '(v0, v1) <- (pargs [Tuntyped; Tuntyped] varg)?;;        
+      mem <- trigger (SGet v_mem);; mem <- mem↓?;;
+      b <- (vcmp mem v0 v1)?;;
+      if b: bool
+      then Ret (Vint 1%Z)
+      else Ret (Vint 0%Z)
+  .
+
+  Context `{Σ: GRA.t}.
+  
+  Definition fnsems : alist string (list string * (Any.t -> itree pmodE Any.t)) :=
+    [(MemName.alloc, ([scope], cfunU alloc)) ;
+     (MemName.free,  ([scope], cfunU free)) ;
+     (MemName.load,  ([scope], cfunU load)) ;
+     (MemName.store, ([scope], cfunU store)) ;
+     (MemName.cmp,   ([scope], cfunU cmp))].
+
+  Variable csl: gname -> bool.
+
+  Program Definition MemSem (sk: Sk.t): PModSem.t :=
+    {|
+      PModSem.scopes := [scope];
+      PModSem.fnsems := fnsems ;
+      PModSem.initial_st := [(v_mem, (Mem.load_mem csl sk)↑)];
+    |}
+  .
+  Solve All Obligations with prove_scope.
+
+  Definition Mem: PMod.t := {|
+    PMod.get_modsem := MemSem;
+    PMod.sk := Sk.unit;
+  |}
+  .
+
+  Definition t : HMod.t := Seal.sealing "ccr" (PMod.to_hmod Mem).
+
+End MEMI.  
+End MemI.
